<?xml version="1.0"?>
<rdf:RDF xmlns="http://purl.obolibrary.org/obo/ecocore/imports/nbo_import.owl#"
     xml:base="http://purl.obolibrary.org/obo/ecocore/imports/nbo_import.owl"
     xmlns:rdf="http://www.w3.org/1999/02/22-rdf-syntax-ns#"
     xmlns:owl="http://www.w3.org/2002/07/owl#"
     xmlns:xml="http://www.w3.org/XML/1998/namespace"
     xmlns:xsd="http://www.w3.org/2001/XMLSchema#"
     xmlns:rdfs="http://www.w3.org/2000/01/rdf-schema#"
     xmlns:obo="http://purl.obolibrary.org/obo/">
    <owl:Ontology rdf:about="http://purl.obolibrary.org/obo/ecocore/imports/nbo_import.owl"/>
    


    <!-- 
    ///////////////////////////////////////////////////////////////////////////////////////
    //
    // Annotation properties
    //
    ///////////////////////////////////////////////////////////////////////////////////////
     -->

    


    <!-- http://purl.obolibrary.org/obo/IAO_0000115 -->

    <owl:AnnotationProperty rdf:about="http://purl.obolibrary.org/obo/IAO_0000115"/>
    


    <!-- 
    ///////////////////////////////////////////////////////////////////////////////////////
    //
    // Classes
    //
    ///////////////////////////////////////////////////////////////////////////////////////
     -->

    


    <!-- http://purl.obolibrary.org/obo/NBO_0000010 -->

    <owl:Class rdf:about="http://purl.obolibrary.org/obo/NBO_0000010">
        <rdfs:subClassOf rdf:resource="http://purl.obolibrary.org/obo/NBO_0000313"/>
        <obo:IAO_0000115>&quot;Behavior related to the actions or interactions of an organism that are associated with reproduction.&quot; [GOC:jl]</obo:IAO_0000115>
        <rdfs:label rdf:datatype="http://www.w3.org/2001/XMLSchema#string">reproductive behavior</rdfs:label>
    </owl:Class>
    


    <!-- http://purl.obolibrary.org/obo/NBO_0000011 -->

    <owl:Class rdf:about="http://purl.obolibrary.org/obo/NBO_0000011">
        <rdfs:subClassOf rdf:resource="http://purl.obolibrary.org/obo/NBO_0000313"/>
        <obo:IAO_0000115>&quot;A behavior that involves two or more individuals.&quot; [Wikipedia:Social_behavior]</obo:IAO_0000115>
        <rdfs:label rdf:datatype="http://www.w3.org/2001/XMLSchema#string">social behavior</rdfs:label>
    </owl:Class>
    


    <!-- http://purl.obolibrary.org/obo/NBO_0000014 -->

    <owl:Class rdf:about="http://purl.obolibrary.org/obo/NBO_0000014">
        <rdfs:subClassOf rdf:resource="http://purl.obolibrary.org/obo/NBO_0000010"/>
        <obo:IAO_0000115>&quot;Behavior related to the interactions between organisms for the purpose of mating.&quot; [NBO:GVG]</obo:IAO_0000115>
        <rdfs:label rdf:datatype="http://www.w3.org/2001/XMLSchema#string">mating behavior</rdfs:label>
    </owl:Class>
    


    <!-- http://purl.obolibrary.org/obo/NBO_0000015 -->

    <owl:Class rdf:about="http://purl.obolibrary.org/obo/NBO_0000015">
        <rdfs:subClassOf rdf:resource="http://purl.obolibrary.org/obo/NBO_0000121"/>
        <obo:IAO_0000115>&quot;A behavioral interaction between organisms in which one organism has the intention of inflicting damage on another individual using physical or verbal means.&quot; [wikipedia:Aggression]</obo:IAO_0000115>
        <rdfs:label rdf:datatype="http://www.w3.org/2001/XMLSchema#string">aggressive behavior</rdfs:label>
    </owl:Class>
    


    <!-- http://purl.obolibrary.org/obo/NBO_0000034 -->

    <owl:Class rdf:about="http://purl.obolibrary.org/obo/NBO_0000034">
        <rdfs:subClassOf rdf:resource="http://purl.obolibrary.org/obo/NBO_0000010"/>
        <obo:IAO_0000115>&quot;Behaviour related to the activity which primary purpose is the sexual reproduction.&quot; [NBO:GVG]</obo:IAO_0000115>
        <rdfs:label rdf:datatype="http://www.w3.org/2001/XMLSchema#string">sexual activity</rdfs:label>
    </owl:Class>
    


    <!-- http://purl.obolibrary.org/obo/NBO_0000060 -->

    <owl:Class rdf:about="http://purl.obolibrary.org/obo/NBO_0000060">
        <rdfs:subClassOf rdf:resource="http://purl.obolibrary.org/obo/NBO_0000034"/>
        <obo:IAO_0000115>&quot;The act of sexual union between male and female, involving the transfer of sperm.&quot; [ISBN:0721662544]</obo:IAO_0000115>
        <rdfs:label rdf:datatype="http://www.w3.org/2001/XMLSchema#string">copulation</rdfs:label>
    </owl:Class>
    


    <!-- http://purl.obolibrary.org/obo/NBO_0000077 -->

    <owl:Class rdf:about="http://purl.obolibrary.org/obo/NBO_0000077">
        <rdfs:subClassOf rdf:resource="http://purl.obolibrary.org/obo/NBO_0000014"/>
        <obo:IAO_0000115>&quot;The behavioral interactions between organisms for the purpose of attracting sexual partners.&quot; [GOC:dph]</obo:IAO_0000115>
        <rdfs:label rdf:datatype="http://www.w3.org/2001/XMLSchema#string">courtship behavior</rdfs:label>
    </owl:Class>
    


    <!-- http://purl.obolibrary.org/obo/NBO_0000078 -->

    <owl:Class rdf:about="http://purl.obolibrary.org/obo/NBO_0000078">
        <rdfs:subClassOf rdf:resource="http://purl.obolibrary.org/obo/NBO_0000010"/>
        <obo:IAO_0000115>&quot;Behavior related to the specific actions or reactions of an organism following mating.&quot; [GOC:bf]</obo:IAO_0000115>
        <rdfs:label rdf:datatype="http://www.w3.org/2001/XMLSchema#string">post-mating behavior</rdfs:label>
    </owl:Class>
    


    <!-- http://purl.obolibrary.org/obo/NBO_0000105 -->

    <owl:Class rdf:about="http://purl.obolibrary.org/obo/NBO_0000105">
        <rdfs:subClassOf rdf:resource="http://purl.obolibrary.org/obo/NBO_0000740"/>
        <obo:IAO_0000115>&quot;Exhibiting a domineering, assault posture and/or hostile physical action towards animals.&quot; [NBO:GVG]</obo:IAO_0000115>
        <rdfs:label rdf:datatype="http://www.w3.org/2001/XMLSchema#string">aggressive behavior towards animals</rdfs:label>
    </owl:Class>
    


    <!-- http://purl.obolibrary.org/obo/NBO_0000121 -->

    <owl:Class rdf:about="http://purl.obolibrary.org/obo/NBO_0000121">
        <rdfs:subClassOf rdf:resource="http://purl.obolibrary.org/obo/NBO_0000011"/>
        <rdfs:subClassOf rdf:resource="http://purl.obolibrary.org/obo/NBO_0000313"/>
        <rdfs:label rdf:datatype="http://www.w3.org/2001/XMLSchema#string">agonistic behavior</rdfs:label>
    </owl:Class>
    


    <!-- http://purl.obolibrary.org/obo/NBO_0000146 -->

    <owl:Class rdf:about="http://purl.obolibrary.org/obo/NBO_0000146">
        <rdfs:subClassOf rdf:resource="http://purl.obolibrary.org/obo/NBO_0000014"/>
        <rdfs:label rdf:datatype="http://www.w3.org/2001/XMLSchema#string">mating receptivity</rdfs:label>
    </owl:Class>
    


    <!-- http://purl.obolibrary.org/obo/NBO_0000147 -->

    <owl:Class rdf:about="http://purl.obolibrary.org/obo/NBO_0000147">
        <rdfs:subClassOf rdf:resource="http://purl.obolibrary.org/obo/NBO_0000014"/>
        <rdfs:label rdf:datatype="http://www.w3.org/2001/XMLSchema#string">sexual display behavior</rdfs:label>
    </owl:Class>
    


    <!-- http://purl.obolibrary.org/obo/NBO_0000285 -->

    <owl:Class rdf:about="http://purl.obolibrary.org/obo/NBO_0000285">
        <rdfs:subClassOf rdf:resource="http://purl.obolibrary.org/obo/NBO_0000286"/>
        <obo:IAO_0000115>&quot;A helping behavior (without expectation of extrinsic rewards and sometimes involving personal risk or sacrifice) that benefits individuals or society.&quot; [NBO:GVG]</obo:IAO_0000115>
        <rdfs:label rdf:datatype="http://www.w3.org/2001/XMLSchema#string">altruism behavior</rdfs:label>
    </owl:Class>
    


    <!-- http://purl.obolibrary.org/obo/NBO_0000286 -->

    <owl:Class rdf:about="http://purl.obolibrary.org/obo/NBO_0000286">
        <rdfs:subClassOf rdf:resource="http://purl.obolibrary.org/obo/NBO_0000011"/>
        <obo:IAO_0000115>&quot;Prosocial behavior is caring about the welfare and rights of others, feeling concern and empathy for them, and acting in ways that benefit others.&quot; [wikipedia:Prosocial_behavior]</obo:IAO_0000115>
        <rdfs:label rdf:datatype="http://www.w3.org/2001/XMLSchema#string">prosocial behavior</rdfs:label>
    </owl:Class>
    


    <!-- http://purl.obolibrary.org/obo/NBO_0000287 -->

    <owl:Class rdf:about="http://purl.obolibrary.org/obo/NBO_0000287">
        <rdfs:subClassOf rdf:resource="http://purl.obolibrary.org/obo/NBO_0000286"/>
        <obo:IAO_0000115>&quot;Helping behavior refers to voluntary actions intended to help the others, with reward regarded or disregarded.&quot; [wikipedia:Helping_behavior]</obo:IAO_0000115>
        <rdfs:label rdf:datatype="http://www.w3.org/2001/XMLSchema#string">helping behavior</rdfs:label>
    </owl:Class>
    


    <!-- http://purl.obolibrary.org/obo/NBO_0000288 -->

    <owl:Class rdf:about="http://purl.obolibrary.org/obo/NBO_0000288">
        <rdfs:subClassOf rdf:resource="http://purl.obolibrary.org/obo/NBO_0000286"/>
        <obo:IAO_0000115>&quot;Reciprocal altruism is the idea that the incentive for an individual to help in the present is based on the expectation of the potential receipt in the future.&quot; [wikipedia:Helping_behavior]</obo:IAO_0000115>
        <rdfs:label rdf:datatype="http://www.w3.org/2001/XMLSchema#string">reciprocal altruism</rdfs:label>
    </owl:Class>
    


    <!-- http://purl.obolibrary.org/obo/NBO_0000313 -->

    <owl:Class rdf:about="http://purl.obolibrary.org/obo/NBO_0000313">
        <obo:IAO_0000115>&quot;The action, reaction, or performance of an organism in response to external or internal stimuli.&quot; [GO:GO\:0007610]</obo:IAO_0000115>
        <rdfs:label rdf:datatype="http://www.w3.org/2001/XMLSchema#string">behavior</rdfs:label>
    </owl:Class>
    


    <!-- http://purl.obolibrary.org/obo/NBO_0000548 -->

    <owl:Class rdf:about="http://purl.obolibrary.org/obo/NBO_0000548">
        <rdfs:subClassOf rdf:resource="http://purl.obolibrary.org/obo/NBO_0000034"/>
        <obo:IAO_0000115>&quot;Behaviour related to the male activity which primary purpose is the sexual reproduction.&quot; [NBO:GVG]</obo:IAO_0000115>
        <rdfs:label rdf:datatype="http://www.w3.org/2001/XMLSchema#string">male sexual activity</rdfs:label>
    </owl:Class>
    


    <!-- http://purl.obolibrary.org/obo/NBO_0000549 -->

    <owl:Class rdf:about="http://purl.obolibrary.org/obo/NBO_0000549">
        <rdfs:subClassOf rdf:resource="http://purl.obolibrary.org/obo/NBO_0000034"/>
        <obo:IAO_0000115>&quot;Behaviour related to the female activity which primary purpose is the sexual reproduction.&quot; [NBO:GVG]</obo:IAO_0000115>
        <rdfs:label rdf:datatype="http://www.w3.org/2001/XMLSchema#string">female sexual activity</rdfs:label>
    </owl:Class>
    


    <!-- http://purl.obolibrary.org/obo/NBO_0000612 -->

    <owl:Class rdf:about="http://purl.obolibrary.org/obo/NBO_0000612">
        <rdfs:subClassOf rdf:resource="http://purl.obolibrary.org/obo/NBO_0000011"/>
        <obo:IAO_0000115>&quot;A social behavior related to the activity of conveying information.&quot; [wikipedia:Communication]</obo:IAO_0000115>
        <rdfs:label rdf:datatype="http://www.w3.org/2001/XMLSchema#string">communication behavior</rdfs:label>
    </owl:Class>
    


    <!-- http://purl.obolibrary.org/obo/NBO_0000613 -->

    <owl:Class rdf:about="http://purl.obolibrary.org/obo/NBO_0000613">
        <rdfs:subClassOf rdf:resource="http://purl.obolibrary.org/obo/NBO_0000612"/>
        <obo:IAO_0000115>&quot;Communication behavior related to the process of conveying meaning in the form of non-word messages through for example gesture, body language or posture; facial expression and eye contact etc.&quot; [wikipedia:.wikipedia.org/wiki/Nonverbal_communication]</obo:IAO_0000115>
        <rdfs:label rdf:datatype="http://www.w3.org/2001/XMLSchema#string">nonverbal communication behavior</rdfs:label>
    </owl:Class>
    


    <!-- http://purl.obolibrary.org/obo/NBO_0000633 -->

    <owl:Class rdf:about="http://purl.obolibrary.org/obo/NBO_0000633">
        <rdfs:subClassOf rdf:resource="http://purl.obolibrary.org/obo/NBO_0000105"/>
        <obo:IAO_0000115>&quot;Aggressive behavior related to the defence of a fixed area against intruders, typically conspecifics.&quot; [GOC:hjd]</obo:IAO_0000115>
        <rdfs:label rdf:datatype="http://www.w3.org/2001/XMLSchema#string">territorial aggressive behavior</rdfs:label>
    </owl:Class>
    


    <!-- http://purl.obolibrary.org/obo/NBO_0000637 -->

    <owl:Class rdf:about="http://purl.obolibrary.org/obo/NBO_0000637">
        <rdfs:subClassOf rdf:resource="http://purl.obolibrary.org/obo/NBO_0000077"/>
        <obo:IAO_0000115>&quot;The actions or reactions of a male, for the purpose of attracting a sexual partner.&quot; [GOC:bf]</obo:IAO_0000115>
        <rdfs:label rdf:datatype="http://www.w3.org/2001/XMLSchema#string">male courtship behavior</rdfs:label>
    </owl:Class>
    


    <!-- http://purl.obolibrary.org/obo/NBO_0000638 -->

    <owl:Class rdf:about="http://purl.obolibrary.org/obo/NBO_0000638">
        <rdfs:subClassOf rdf:resource="http://purl.obolibrary.org/obo/NBO_0000077"/>
        <obo:IAO_0000115>&quot;The actions or reactions of a female, for the purpose of attracting a sexual partner.&quot; [GOC:bf]</obo:IAO_0000115>
        <rdfs:label rdf:datatype="http://www.w3.org/2001/XMLSchema#string">female courtship behavior</rdfs:label>
    </owl:Class>
    


    <!-- http://purl.obolibrary.org/obo/NBO_0000740 -->

    <owl:Class rdf:about="http://purl.obolibrary.org/obo/NBO_0000740">
        <rdfs:subClassOf rdf:resource="http://purl.obolibrary.org/obo/NBO_0000015"/>
        <rdfs:label rdf:datatype="http://www.w3.org/2001/XMLSchema#string">aggressive behavior by intent</rdfs:label>
    </owl:Class>
    


    <!-- http://purl.obolibrary.org/obo/NBO_0000743 -->

    <owl:Class rdf:about="http://purl.obolibrary.org/obo/NBO_0000743">
        <rdfs:subClassOf rdf:resource="http://purl.obolibrary.org/obo/NBO_0000105"/>
        <rdfs:subClassOf rdf:resource="http://purl.obolibrary.org/obo/NBO_0000121"/>
        <obo:IAO_0000115>&quot;An aggressive behavior towards other members of the society.&quot; [NBO:RH]</obo:IAO_0000115>
        <rdfs:label rdf:datatype="http://www.w3.org/2001/XMLSchema#string">social aggression behavior</rdfs:label>
    </owl:Class>
</rdf:RDF>



<!-- Generated by the OWL API (version 4.2.6) https://github.com/owlcs/owlapi -->

